matches_map_group_map_group_cons_zero_or_one_deterministically_encoded_cbor_map_key_order

src/cbor/CDDL.Spec.fst
@@ -873,3 +873,135 @@ let matches_map_group_map_group_cons_one_no_repeats
         (fun prf -> matches_map_group_map_group_cons_restricted_some_no_repeats_intro k ty true g x prf)
         (fun prf -> matches_map_group_map_group_cons_restricted_some_no_repeats_elim k ty true g x prf)
     else ()
+
+let rec list_for_all_weaken
+  (#t: Type)
+  (p1: t -> bool)
+  (p2: t -> bool { forall x . p1 x ==> p2 x })
+  (l: list t)
+: Lemma
+  (requires (List.Tot.for_all p1 l))
+  (ensures (List.Tot.for_all p2 l))
+= match l with
+  | [] -> ()
+  | _ :: q -> list_for_all_weaken p1 p2 q
+
+let rec list_sorted_cons_elim
+  (#t1: Type)
+  (key_order: t1 -> t1 -> bool {
+    forall x y z . (key_order x y /\ key_order y z) ==> key_order x z
+  })
+  (a: t1)
+  (q: list t1)
+: Lemma
+  (requires (List.Tot.sorted key_order (a :: q)))
+  (ensures (List.Tot.for_all (key_order a) q))
+  (decreases q)
+= match q with
+  | [] -> ()
+  | b :: r ->
+    list_sorted_cons_elim key_order b r;
+    list_for_all_weaken (key_order b) (key_order a) r
+
+let rec list_sorted_filter
+  (#t1: Type)
+  (key_order: t1 -> t1 -> bool {
+    forall x y z . (key_order x y /\ key_order y z) ==> key_order x z
+  })
+  (f: t1 -> bool)
+  (l: list t1)
+: Lemma
+  (requires (
+    List.Tot.sorted key_order l
+  ))
+  (ensures (
+    List.Tot.sorted key_order (List.Tot.filter f l)
+  ))
+= match l with
+  | [] -> ()
+  | a :: q ->
+    list_sorted_filter key_order f q;
+    if f a
+    then begin
+      list_sorted_cons_elim key_order a q;
+      list_for_all_filter_invariant (key_order a) f q
+    end
+    else ()
+
+let list_sorted_deterministically_encoded_cbor_map_key_order_filter
+  (#t: Type)
+  (f: (Cbor.raw_data_item & t) -> bool)
+  (l: list (Cbor.raw_data_item & t))
+: Lemma
+  (requires (
+    List.Tot.sorted (Cbor.map_entry_order Cbor.deterministically_encoded_cbor_map_key_order _) l
+  ))
+  (ensures (
+    List.Tot.sorted (Cbor.map_entry_order Cbor.deterministically_encoded_cbor_map_key_order _) (List.Tot.filter f l)
+  ))
+  [SMTPat (List.Tot.sorted (Cbor.map_entry_order Cbor.deterministically_encoded_cbor_map_key_order _) (List.Tot.filter f l))]
+= list_sorted_filter (Cbor.map_entry_order Cbor.deterministically_encoded_cbor_map_key_order _) f l
+
+let rec list_sorted_map_entry_order_lt_tail
+  (#t1 #t2: Type)
+  (key_order: t1 -> t1 -> bool {
+    (forall x y z . (key_order x y /\ key_order y z) ==> key_order x z)
+  })
+  (a: (t1 & t2))
+  (l: list (t1 & t2))
+  (k: t1)
+: Lemma
+  (requires (List.Tot.sorted (Cbor.map_entry_order key_order _) (a :: l) /\ List.Tot.memP k (List.Tot.map fst l)))
+  (ensures (key_order (fst a) k))
+  (decreases l)
+= let b :: q = l in
+  if FStar.StrongExcludedMiddle.strong_excluded_middle (k == fst b)
+  then ()
+  else list_sorted_map_entry_order_lt_tail key_order b q k
+
+let list_sorted_map_entry_order_not_memP_tail
+  (#t1 #t2: Type)
+  (key_order: t1 -> t1 -> bool {
+    (forall x . key_order x x == false) /\
+    (forall x y z . (key_order x y /\ key_order y z) ==> key_order x z)
+  })
+  (a: (t1 & t2))
+  (l: list (t1 & t2))
+: Lemma
+  (requires (List.Tot.sorted (Cbor.map_entry_order key_order _) (a :: l)))
+  (ensures (~ (List.Tot.memP (fst a) (List.Tot.map fst l))))
+= Classical.move_requires (list_sorted_map_entry_order_lt_tail key_order a l) (fst a)
+
+let rec list_sorted_map_entry_order_no_repeats
+  (#t1 #t2: Type)
+  (key_order: t1 -> t1 -> bool {
+    (forall x . key_order x x == false) /\
+    (forall x y z . (key_order x y /\ key_order y z) ==> key_order x z)
+  })
+  (l: list (t1 & t2))
+: Lemma
+  (requires (List.Tot.sorted (Cbor.map_entry_order key_order _) l))
+  (ensures (List.Tot.no_repeats_p (List.Tot.map fst l)))
+= match l with
+  | [] -> ()
+  | a :: q ->
+    list_sorted_map_entry_order_no_repeats key_order q;
+    list_sorted_map_entry_order_not_memP_tail key_order a q
+
+let list_sorted_map_entry_order_deterministically_encoded_cbor_map_key_order_no_repeats
+  (#t: Type)
+  (l: list (Cbor.raw_data_item & t))
+: Lemma
+  (requires (List.Tot.sorted (Cbor.map_entry_order Cbor.deterministically_encoded_cbor_map_key_order _) l))
+  (ensures (List.Tot.no_repeats_p (List.Tot.map fst l)))
+= list_sorted_map_entry_order_no_repeats Cbor.deterministically_encoded_cbor_map_key_order l
+
+let matches_map_group_map_group_cons_zero_or_one_deterministically_encoded_cbor_map_key_order
+  #b k ty g x
+= list_sorted_map_entry_order_deterministically_encoded_cbor_map_key_order_no_repeats x;
+  matches_map_group_map_group_cons_zero_or_one_no_repeats k ty g x
+
+let matches_map_group_map_group_cons_one_deterministically_encoded_cbor_map_key_order
+  #b k ty g x
+= list_sorted_map_entry_order_deterministically_encoded_cbor_map_key_order_no_repeats x;
+  matches_map_group_map_group_cons_one_no_repeats k ty g x
